code/ecdsap256/Hacl.Impl.P256.PointAdd.fst
@@ -40,82 +40,86 @@ val lemma_pointAddToSpecification:
   h: nat -> r: nat -> 
   Lemma
     (requires (    
-      let x3D, y3D, z3D = fromDomain_ x3, fromDomain_ y3, fromDomain_ z3 in 
 
-      let u1D, u2D = fromDomain_ u1, fromDomain_ u2 in 
-      let s1D, s2D = fromDomain_ s1, fromDomain_ s2 in 
-      let rD = fromDomain_ r in    
-      let hD = fromDomain_ h in 
-     
-      u1 == toDomain_ (qzD * qzD * pxD % prime256) /\
-      u2 == toDomain_ (pzD * pzD * qxD % prime256) /\
-      s1 == toDomain_ (qzD * qzD * qzD * pyD % prime256) /\
-      s2 == toDomain_ (pzD * pzD * pzD * qyD % prime256) /\
+      let prime = getPrime c in 
       
-      h == toDomain_ ((u2D - u1D) % prime256) /\
-      r == toDomain_ ((s2D - s1D) % prime256) /\
+      let x3D, y3D, z3D = fromDomain_ #c x3, fromDomain_ #c y3, fromDomain_ #c z3 in 
+
+      let u1D, u2D = fromDomain_ #c u1, fromDomain_ #c u2 in 
+      let s1D, s2D = fromDomain_ #c s1, fromDomain_ #c s2 in 
+      let rD = fromDomain_ #c r in    
+      let hD = fromDomain_ #c h in 
+     
+      u1 == toDomain_ #c (qzD * qzD * pxD % prime256) /\
+      u2 == toDomain_ #c (pzD * pzD * qxD % prime256) /\
+      s1 == toDomain_ #c (qzD * qzD * qzD * pyD % prime256) /\
+      s2 == toDomain_ #c (pzD * pzD * pzD * qyD % prime256) /\
+      
+      h == toDomain_ #c ((u2D - u1D) % prime256) /\
+      r == toDomain_ #c ((s2D - s1D) % prime256) /\
       (
   if qzD = 0 then 
-    fromDomain_ x3 == pxD /\ fromDomain_ y3 == pyD /\ fromDomain_ z3 == pzD
+    fromDomain_ #c x3 == pxD /\ fromDomain_ #c y3 == pyD /\ fromDomain_ #c z3 == pzD
   else if pzD = 0 then 
-      fromDomain_ x3 == qxD /\  fromDomain_ y3 == qyD /\  fromDomain_ z3 == qzD 
+      fromDomain_ #c x3  == qxD /\  fromDomain_ #c y3 == qyD /\ fromDomain_ #c z3 == qzD 
   else
-      x3 == toDomain_ ((rD * rD - hD * hD * hD - 2 * hD * hD * u1D) % prime) /\
-      y3 == toDomain_ (((hD * hD * u1D - x3D) * rD - s1D * hD*hD*hD) % prime) /\
-      z3 == toDomain_ ((pzD * qzD * hD) % prime)
+      x3 == toDomain_ #c ((rD * rD - hD * hD * hD - 2 * hD * hD * u1D) % prime) /\
+      y3 == toDomain_ #c (((hD * hD * u1D - x3D) * rD - s1D * hD*hD*hD) % prime) /\
+      z3 == toDomain_ #c ((pzD * qzD * hD) % prime)
   )
       )
   )
   (ensures 
   (    
-    let x3D, y3D, z3D = fromDomain_ x3, fromDomain_ y3, fromDomain_ z3 in 
-    let (xN, yN, zN) = _point_add #P256 (pxD, pyD, pzD) (qxD, qyD, qzD) in
-    let u1D = fromDomain_ u1 in let u2D = fromDomain_ u2 in 
-    let s1D = fromDomain_ s1 in let s2D = fromDomain_ s2 in 
+    let x3D, y3D, z3D = fromDomain_ #c x3, fromDomain_ #c y3, fromDomain_ #c z3 in 
+    let (xN, yN, zN) = _point_add #c (pxD, pyD, pzD) (qxD, qyD, qzD) in
+    let u1D = fromDomain_ #c u1 in let u2D = fromDomain_ #c u2 in 
+    let s1D = fromDomain_ #c s1 in let s2D = fromDomain_ #c s2 in 
     xN == x3D /\  yN == y3D /\ zN == z3D
   )
 )
 
-let lemma_pointAddToSpecification x1D y1D z1D x2D y2D z2D x3 y3 z3  u1 u2 s1 s2 h r = 
+let lemma_pointAddToSpecification #c x1D y1D z1D x2D y2D z2D x3 y3 z3  u1 u2 s1 s2 h r = 
   let open FStar.Tactics in 
   let open FStar.Tactics.Canon in 
    
-  let u1D = fromDomain_ u1 in 
-  let u2D = fromDomain_ u2 in 
-  let s1D = fromDomain_ s1 in 
-  let s2D = fromDomain_ s2 in 
+  let u1D = fromDomain_ #c u1 in 
+  let u2D = fromDomain_ #c u2 in 
+  let s1D = fromDomain_ #c s1 in 
+  let s2D = fromDomain_ #c s2 in 
 
-  let hD = fromDomain_ h in 
-  let rD = fromDomain_ r in 
+  let hD = fromDomain_ #c h in 
+  let rD = fromDomain_ #c r in 
 
-  let x3D, y3D, z3D = fromDomain_ x3, fromDomain_ y3, fromDomain_ z3 in 
+  let x3D, y3D, z3D = fromDomain_ #c x3, fromDomain_ #c y3, fromDomain_ #c z3 in 
 
   let pxD, pyD, pzD = x1D, y1D, z1D in 
   let qxD, qyD, qzD = x2D, y2D, z2D in 
 
      assert(
-        
 
-      u1 == toDomain_ (z2D * z2D * pxD % prime256) /\
-      u2 == toDomain_ (pzD * pzD * qxD % prime256) /\
-      s1 == toDomain_ (qzD * qzD * qzD * pyD % prime256) /\
-      s2 == toDomain_ (pzD * pzD * pzD * qyD % prime256) /\
+     let prime = getPrime c in 
+
+      u1 == toDomain_ #c (z2D * z2D * pxD % prime256) /\
+      u2 == toDomain_ #c (pzD * pzD * qxD % prime256) /\
+      s1 == toDomain_ #c (qzD * qzD * qzD * pyD % prime256) /\
+      s2 == toDomain_ #c (pzD * pzD * pzD * qyD % prime256) /\
       
-      h == toDomain_ ((u2D - u1D) % prime256) /\
-      r == toDomain_ ((s2D - s1D) % prime256) /\
+      h == toDomain_ #c ((u2D - u1D) % prime256) /\
+      r == toDomain_ #c ((s2D - s1D) % prime256) /\
       (
   if qzD = 0 then 
      x3D == pxD /\ y3D == pyD /\  z3D == pzD
   else if pzD = 0 then 
        x3D == qxD /\ y3D == qyD /\ z3D == qzD 
   else
-      x3 == toDomain_ ((rD * rD - hD * hD * hD - 2 * hD * hD * u1D) % prime) /\
-      y3 == toDomain_ (((hD * hD * u1D - x3D) * rD - s1D * hD * hD * hD) % prime) /\
-      z3 == toDomain_ ((pzD * qzD * hD) % prime)
+      x3 == toDomain_ #c ((rD * rD - hD * hD * hD - 2 * hD * hD * u1D) % prime) /\
+      y3 == toDomain_ #c (((hD * hD * u1D - x3D) * rD - s1D * hD * hD * hD) % prime) /\
+      z3 == toDomain_ #c ((pzD * qzD * hD) % prime)
   )
       );
 
-    let (xN, yN, zN) = _point_add #P256 (x1D, y1D, z1D) (x2D, y2D, z2D) in 
+    let (xN, yN, zN) = _point_add #c (x1D, y1D, z1D) (x2D, y2D, z2D) in 
 
 
     assert_by_tactic (z2D * z2D * pxD = pxD * (z2D * z2D)) canon; 
@@ -193,29 +197,39 @@ let lemma_point_add_1 a b c d e =
 
 
 
-val copy_point_conditional: x3_out: felem -> y3_out: felem -> z3_out: felem -> p: point -> maskPoint: point -> Stack unit
+val copy_point_conditional: #c: curve ->  x3_out: felem c -> y3_out: felem c -> z3_out: felem c -> p: point c -> maskPoint: point c -> Stack unit
   (requires fun h -> live h x3_out /\ live h y3_out /\ live h z3_out /\ live h p /\ live h maskPoint /\ 
     LowStar.Monotonic.Buffer.all_disjoint[loc x3_out; loc y3_out; loc z3_out; loc p; loc maskPoint] /\
-    as_nat h x3_out < prime /\ as_nat h y3_out < prime /\ as_nat h z3_out < prime /\
-    as_nat h (gsub p (size 0) (size 4)) < prime /\ 
-    as_nat h (gsub p (size 4) (size 4)) < prime /\ 
-    as_nat h (gsub p (size 8) (size 4)) < prime 
+      (
+	let prime = getPrime c in 
+	as_nat c h x3_out < prime /\ as_nat c h y3_out < prime /\ as_nat c h z3_out < prime /\
+	as_nat c h (gsub p (size 0) (size 4)) < prime /\ 
+	as_nat c h (gsub p (size 4) (size 4)) < prime /\ 
+	as_nat c h (gsub p (size 8) (size 4)) < prime 
+    )
   )
   (ensures fun h0 _ h1 -> modifies (loc x3_out |+| loc y3_out |+| loc z3_out) h0 h1 /\ 
-    as_nat h1 x3_out < prime /\
-    as_nat h1 y3_out < prime /\
-    as_nat h1 z3_out < prime /\
     (
-      let mask = as_nat h0 (gsub maskPoint (size 8) (size 4)) in 
+      let prime = getPrime c in 
+    as_nat c h1 x3_out < prime /\
+    as_nat c h1 y3_out < prime /\
+    as_nat c h1 z3_out < prime /\
+    (
+      let mask = as_nat c h0 (gsub maskPoint (size 8) (size 4)) in 
       let x = gsub p (size 0) (size 4) in 
       let y = gsub p (size 4) (size 4) in 
       let z = gsub p (size 8) (size 4) in 
 
       if mask = 0 then 
-	as_nat h1 x3_out == as_nat h0 x /\ as_nat h1 y3_out == as_nat h0 y /\ as_nat h1 z3_out == as_nat h0 z
+	as_nat c h1 x3_out == as_nat c h0 x /\ 
+	as_nat c h1 y3_out == as_nat c h0 y /\ 
+	as_nat c h1 z3_out == as_nat c h0 z
       else 
-	as_nat h1 x3_out == as_nat h0 x3_out /\ as_nat h1 y3_out == as_nat h0 y3_out /\ as_nat h1 z3_out == as_nat h0 z3_out
+	as_nat c h1 x3_out == as_nat c h0 x3_out /\ 
+	as_nat c h1 y3_out == as_nat c h0 y3_out /\ 
+	as_nat c h1 z3_out == as_nat c h0 z3_out
     )
+   )
 )
 
 let copy_point_conditional x3_out y3_out z3_out p maskPoint = 
@@ -232,35 +246,41 @@ let copy_point_conditional x3_out y3_out z3_out p maskPoint =
 
     
 inline_for_extraction noextract 
-val move_from_jacobian_coordinates: u1: felem -> u2: felem -> s1: felem -> s2: felem ->  p: point -> q: point -> 
+val move_from_jacobian_coordinates: #c: curve -> u1: felem c -> u2: felem c -> s1: felem c -> s2: felem c -> p: point c -> q: point c -> 
   tempBuffer16: lbuffer uint64 (size 16) -> 
   Stack unit (requires fun h -> live h u1 /\ live h u2 /\ live h s1 /\ live h s2 /\ live h p /\ live h q /\ live h tempBuffer16 /\
    LowStar.Monotonic.Buffer.all_disjoint [loc tempBuffer16; loc p; loc q; loc u1; loc u2; loc s1; loc s2] /\
-    as_nat h (gsub p (size 8) (size 4)) < prime /\ 
-    as_nat h (gsub p (size 0) (size 4)) < prime /\ 
-    as_nat h (gsub p (size 4) (size 4)) < prime /\
-    as_nat h (gsub q (size 8) (size 4)) < prime /\ 
-    as_nat h (gsub q (size 0) (size 4)) < prime /\ 
-    as_nat h (gsub q (size 4) (size 4)) < prime
+     (
+       let prime = getPrime c in 
+       as_nat c h (gsub p (size 8) (size 4)) < prime /\ 
+       as_nat c h (gsub p (size 0) (size 4)) < prime /\ 
+       as_nat c h (gsub p (size 4) (size 4)) < prime /\
+       as_nat c h (gsub q (size 8) (size 4)) < prime /\ 
+       as_nat c h (gsub q (size 0) (size 4)) < prime /\ 
+       as_nat c h (gsub q (size 4) (size 4)) < prime
+     )
     )
   (ensures fun h0 _ h1 ->  
     modifies (loc u1 |+| loc u2 |+| loc s1 |+| loc s2 |+| loc tempBuffer16) h0 h1 /\
-    as_nat h1 u1 < prime /\ as_nat h1 u2 < prime /\ as_nat h1 s1 < prime /\ as_nat h1 s2 < prime  /\
-    (
-      let pX, pY, pZ = as_nat h0 (gsub p (size 0) (size 4)), as_nat h0 (gsub p (size 4) (size 4)), as_nat h0 (gsub p (size 8) (size 4)) in 
-      let qX, qY, qZ = as_nat h0 (gsub q (size 0) (size 4)), as_nat h0 (gsub q (size 4) (size 4)), as_nat h0 (gsub q (size 8) (size 4)) in 
+      (
+	let prime = getPrime c in 
+	as_nat c h1 u1 < prime /\ as_nat c h1 u2 < prime /\ as_nat c h1 s1 < prime /\ as_nat c h1 s2 < prime  /\
+	(
+	let pX, pY, pZ = as_nat c h0 (gsub p (size 0) (size 4)), as_nat c h0 (gsub p (size 4) (size 4)), as_nat c h0 (gsub p (size 8) (size 4)) in 
+	let qX, qY, qZ = as_nat c h0 (gsub q (size 0) (size 4)), as_nat c h0 (gsub q (size 4) (size 4)), as_nat c h0 (gsub q (size 8) (size 4)) in 
       
-      let pxD, pyD, pzD = fromDomain_ pX, fromDomain_ pY, fromDomain_ pZ in 
-      let qxD, qyD, qzD = fromDomain_ qX, fromDomain_ qY, fromDomain_ qZ in 
+      let pxD, pyD, pzD = fromDomain_ #c pX, fromDomain_ #c pY, fromDomain_ #c pZ in 
+      let qxD, qyD, qzD = fromDomain_ #c qX, fromDomain_ #c qY, fromDomain_ #c qZ in 
 
-      as_nat h1 u1 == toDomain_ (qzD * qzD * pxD % prime256) /\
-      as_nat h1 u2 == toDomain_ (pzD * pzD * qxD % prime256) /\
-      as_nat h1 s1 == toDomain_ (qzD * qzD * qzD * pyD % prime256) /\
-      as_nat h1 s2 == toDomain_ (pzD * pzD * pzD * qyD % prime256)
+      as_nat c h1 u1 == toDomain_ #c (qzD * qzD * pxD % prime256) /\
+      as_nat c h1 u2 == toDomain_ #c (pzD * pzD * qxD % prime256) /\
+      as_nat c h1 s1 == toDomain_ #c (qzD * qzD * qzD * pyD % prime256) /\
+      as_nat c h1 s2 == toDomain_ #c (pzD * pzD * pzD * qyD % prime256)
+   )
 )
 )
 
-let move_from_jacobian_coordinates u1 u2 s1 s2 p q tempBuffer = 
+let move_from_jacobian_coordinates #c u1 u2 s1 s2 p q tempBuffer = 
     let h0 = ST.get() in 
    let pX = sub p (size 0) (size 4) in 
    let pY = sub p (size 4) (size 4) in 
@@ -285,39 +305,53 @@ let move_from_jacobian_coordinates u1 u2 s1 s2 p q tempBuffer =
    
    montgomery_multiplication_buffer z2Cube pY s1;
    montgomery_multiplication_buffer z1Cube qY s2;
-   
+   () (*
 
-     lemma_mod_mul_distr_l (fromDomain_ (as_nat h0 qZ) * fromDomain_ (as_nat h0 qZ)) (fromDomain_ (as_nat h0 qZ)) prime256;
+     lemma_mod_mul_distr_l (fromDomain_ #c (as_nat c h0 qZ) * fromDomain_ #c (as_nat h0 qZ)) (fromDomain_ (as_nat h0 qZ)) prime256;
      lemma_mod_mul_distr_l (fromDomain_ (as_nat h0 pZ) * fromDomain_ (as_nat h0 pZ)) (fromDomain_ (as_nat h0 pZ)) prime256;
      lemma_mod_mul_distr_l (fromDomain_ (as_nat h0 qZ) * fromDomain_ (as_nat h0 qZ)) (fromDomain_ (as_nat h0 pX)) prime256;   
      
      lemma_mod_mul_distr_l (fromDomain_ (as_nat h0 pZ) * fromDomain_ (as_nat h0 pZ)) (fromDomain_ (as_nat h0 qX)) prime256;
      lemma_mod_mul_distr_l (fromDomain_ (as_nat h0 qZ) * fromDomain_ (as_nat h0 qZ) * fromDomain_ (as_nat h0 qZ)) (fromDomain_ (as_nat h0 pY)) prime256;
-     lemma_mod_mul_distr_l (fromDomain_ (as_nat h0 pZ) * fromDomain_ (as_nat h0 pZ) * fromDomain_ (as_nat h0 pZ)) (fromDomain_ (as_nat h0 qY)) prime256
+     lemma_mod_mul_distr_l (fromDomain_ (as_nat h0 pZ) * fromDomain_ (as_nat h0 pZ) * fromDomain_ (as_nat h0 pZ)) (fromDomain_ (as_nat h0 qY)) prime256 *)
 
 
 
 inline_for_extraction noextract 
-val compute_common_params_point_add: h: felem -> r: felem -> uh: felem -> hCube: felem -> 
-  u1: felem -> u2: felem -> s1: felem -> s2: felem -> tempBuffer: lbuffer uint64 (size 16) -> 
+val compute_common_params_point_add: #c: curve -> h: felem c -> r: felem c -> uh: felem c -> hCube: felem c -> 
+  u1: felem c -> u2: felem c -> s1: felem c -> s2: felem c -> tempBuffer: lbuffer uint64 (size 16) -> 
   Stack unit 
     (requires fun h0 -> live h0 h /\ live h0 r /\ live h0 uh /\ live h0 hCube /\ live h0 u1 /\ live h0 u2 /\ live h0 s1 /\ live h0 s2 /\ live h0 tempBuffer /\  
-      LowStar.Monotonic.Buffer.all_disjoint [loc u1; loc u2; loc s1; loc s2; loc h; loc r; loc uh; loc hCube; loc tempBuffer] /\ as_nat h0 u1 < prime /\ as_nat h0 u2 < prime /\ as_nat h0 s1 < prime /\ as_nat h0 s2 < prime)
+      LowStar.Monotonic.Buffer.all_disjoint [loc u1; loc u2; loc s1; loc s2; loc h; loc r; loc uh; loc hCube; loc tempBuffer] /\ 
+      (
+	let prime = getPrime c in 
+	as_nat c h0 u1 < prime /\ 
+	as_nat c h0 u2 < prime /\ 
+	as_nat c h0 s1 < prime /\ 
+	as_nat c h0 s2 < prime)
+)
     (ensures fun h0 _ h1 ->  
       modifies (loc h |+| loc r |+| loc uh |+| loc hCube |+| loc tempBuffer) h0 h1 /\ 
-      as_nat h1 h < prime /\ as_nat h1 r < prime /\ as_nat h1 uh < prime /\ as_nat h1 hCube < prime /\
-      (
-	let u1D = fromDomain_ (as_nat h0 u1) in 
-	let u2D = fromDomain_ (as_nat h0 u2) in 
-	let s1D = fromDomain_ (as_nat h0 s1) in 
-	let s2D = fromDomain_ (as_nat h0 s2) in 
-	
-	let hD = fromDomain_ (as_nat h1 h) in 
 
-	as_nat h1 h == toDomain_ ((u2D - u1D) % prime256) /\
-	as_nat h1 r == toDomain_ ((s2D - s1D) % prime256) /\
-	as_nat h1 uh == toDomain_ (hD * hD * u1D % prime256) /\
-	as_nat h1 hCube == toDomain_ (hD * hD * hD % prime256)
+    (
+      let prime = getPrime c in 
+      as_nat c h1 h < prime /\ 
+      as_nat c h1 r < prime /\ 
+      as_nat c h1 uh < prime /\ 
+      as_nat c h1 hCube < prime /\
+      (
+	let u1D = fromDomain_ #c (as_nat c h0 u1) in 
+	let u2D = fromDomain_ #c (as_nat c h0 u2) in 
+	let s1D = fromDomain_ #c (as_nat c h0 s1) in 
+	let s2D = fromDomain_ #c (as_nat c h0 s2) in 
+	
+	let hD = fromDomain_ #c (as_nat c h1 h) in 
+
+	as_nat c h1 h == toDomain_ #c ((u2D - u1D) % prime256) /\
+	as_nat c h1 r == toDomain_ #c ((s2D - s1D) % prime256) /\
+	as_nat c h1 uh == toDomain_ #c (hD * hD * u1D % prime256) /\
+	as_nat c h1 hCube == toDomain_ #c (hD * hD * hD % prime256)
+	)
   )
 )
 
@@ -332,28 +366,31 @@ let compute_common_params_point_add h r uh hCube u1 u2 s1 s2 tempBuffer =
   montgomery_square_buffer h temp;
     let h3 = ST.get() in   
   montgomery_multiplication_buffer temp u1 uh;
-  montgomery_multiplication_buffer temp h hCube;
+  montgomery_multiplication_buffer temp h hCube; () (*
 
-    lemma_mod_mul_distr_l (fromDomain_ (as_nat h2 h) * fromDomain_ (as_nat h2 h)) (fromDomain_ (as_nat h3 u1)) prime256;
-    lemma_mod_mul_distr_l (fromDomain_ (as_nat h2 h) * fromDomain_ (as_nat h2 h)) (fromDomain_ (as_nat h1 h)) prime256
+    lemma_mod_mul_distr_l (fromDomain_ (as_nat c h2 h) * fromDomain_ (as_nat h2 h)) (fromDomain_ (as_nat h3 u1)) prime256;
+    lemma_mod_mul_distr_l (fromDomain_ (as_nat h2 h) * fromDomain_ (as_nat h2 h)) (fromDomain_ (as_nat h1 h)) prime256 *)
 
 
 inline_for_extraction noextract 
-val computeX3_point_add: x3: felem -> hCube: felem -> uh: felem -> r: felem -> tempBuffer: lbuffer uint64 (size 16)->  Stack unit 
+val computeX3_point_add: #c : curve -> x3: felem c -> hCube: felem c -> uh: felem c -> r: felem c -> tempBuffer: lbuffer uint64 (size 16)->  Stack unit 
   (requires fun h0 -> live h0 x3 /\ live h0 hCube /\ live h0 uh /\ live h0 r /\ live h0 tempBuffer /\
     LowStar.Monotonic.Buffer.all_disjoint [loc x3; loc hCube; loc uh; loc r; loc tempBuffer] /\
-    as_nat h0 hCube < prime /\as_nat h0 uh < prime /\ as_nat h0 r < prime
-  )
-  (ensures fun h0 _ h1 -> modifies (loc x3 |+| loc tempBuffer) h0 h1 /\ as_nat h1 x3 < prime /\ 
     (
-      let hCubeD = fromDomain_ (as_nat h0 hCube) in 
-      let uhD = fromDomain_ (as_nat h0 uh) in 
-      let rD = fromDomain_ (as_nat h0 r) in 
-      as_nat h1 x3 == toDomain_ ((rD * rD - hCubeD - 2 * uhD) % prime256)
+      let prime = getPrime c in 
+      as_nat c h0 hCube < prime /\as_nat c h0 uh < prime /\ as_nat c h0 r < prime)
+      
+  )
+  (ensures fun h0 _ h1 -> modifies (loc x3 |+| loc tempBuffer) h0 h1 /\ as_nat c h1 x3 < getPrime c /\ 
+    (
+      let hCubeD = fromDomain_ #c (as_nat c h0 hCube) in 
+      let uhD = fromDomain_ #c (as_nat c h0 uh) in 
+      let rD = fromDomain_ #c (as_nat c h0 r) in 
+      as_nat c h1 x3 == toDomain_ #c ((rD * rD - hCubeD - 2 * uhD) % prime256)
     )  
   )
 
-let computeX3_point_add x3 hCube uh r tempBuffer = 
+let computeX3_point_add #c x3 hCube uh r tempBuffer = 
     let h0 = ST.get() in 
   let rSquare = sub tempBuffer (size 0) (size 4) in 
   let rH = sub tempBuffer (size 4) (size 4) in 
@@ -364,28 +401,36 @@ let computeX3_point_add x3 hCube uh r tempBuffer =
     let h2 = ST.get() in 
   multByTwo uh twoUh;
     let h3 = ST.get() in 
-  p256_sub rH twoUh x3;  
-  
-    lemma_mod_add_distr (-fromDomain_ (as_nat h1 hCube)) (fromDomain_ (as_nat h0 r) * fromDomain_ (as_nat h0 r)) prime256;
+  p256_sub rH twoUh x3;  ()
+  (*
+    lemma_mod_add_distr (-fromDomain_  (as_nat c h1 hCube)) (fromDomain_ (as_nat c h0 r) * fromDomain_ (as_nat h0 r)) prime256;
     lemma_mod_add_distr (-fromDomain_ (as_nat h3 twoUh)) (fromDomain_ (as_nat h0 r) * fromDomain_ (as_nat h0 r) - fromDomain_ (as_nat h1 hCube)) prime256;
-    lemma_mod_sub_distr (fromDomain_ (as_nat h0 r) * fromDomain_ (as_nat h0 r) - fromDomain_ (as_nat h1 hCube)) (2 * fromDomain_ (as_nat h2 uh)) prime256
+    lemma_mod_sub_distr (fromDomain_ (as_nat h0 r) * fromDomain_ (as_nat h0 r) - fromDomain_ (as_nat h1 hCube)) (2 * fromDomain_ (as_nat h2 uh)) prime256 *)
 
 
 inline_for_extraction noextract 
-val computeY3_point_add:y3: felem -> s1: felem -> hCube: felem -> uh: felem -> x3_out: felem -> r: felem -> tempBuffer: lbuffer uint64 (size 16) -> 
+val computeY3_point_add: #c: curve -> y3: felem c -> s1: felem c -> 
+  hCube: felem c -> uh: felem c -> x3_out: felem c -> r: felem c -> tempBuffer: lbuffer uint64 (size 16) -> 
   Stack unit 
     (requires fun h -> live h y3 /\ live h s1 /\ live h hCube /\ live h uh /\ live h x3_out /\ live h r /\ live h tempBuffer /\
       LowStar.Monotonic.Buffer.all_disjoint [loc y3; loc s1; loc hCube; loc uh; loc x3_out; loc r; loc tempBuffer] /\
-      as_nat h s1 < prime /\ as_nat h hCube < prime /\ as_nat h uh < prime /\ as_nat h x3_out <prime /\ as_nat h r < prime)
+	(let prime  = getPrime c in 
+	  as_nat c h s1 < prime /\ 
+	  as_nat c h hCube < prime /\
+	  as_nat c h uh < prime /\ 
+	  as_nat c h x3_out <prime /\ 
+	  as_nat c h r < prime
+)
+)
     (ensures fun h0 _ h1 -> 
-      modifies (loc y3 |+| loc tempBuffer) h0 h1 /\ as_nat h1 y3 < prime /\ 
+      modifies (loc y3 |+| loc tempBuffer) h0 h1 /\ as_nat c h1 y3 < getPrime c /\ 
       (
-	let s1D = fromDomain_ (as_nat h0 s1) in 
-	let hCubeD = fromDomain_ (as_nat h0 hCube) in 
-	let uhD = fromDomain_ (as_nat h0 uh) in 
-	let x3D = fromDomain_ (as_nat h0 x3_out) in 
-	let rD = fromDomain_ (as_nat h0 r) in 
-	as_nat h1 y3 = toDomain_ (((uhD - x3D) * rD - s1D * hCubeD) % prime256)
+	let s1D = fromDomain_ #c (as_nat c h0 s1) in 
+	let hCubeD = fromDomain_ #c (as_nat c h0 hCube) in 
+	let uhD = fromDomain_ #c (as_nat c h0 uh) in 
+	let x3D = fromDomain_ #c (as_nat c h0 x3_out) in 
+	let rD = fromDomain_ #c (as_nat c h0 r) in 
+	as_nat c h1 y3 = toDomain_ #c (((uhD - x3D) * rD - s1D * hCubeD) % prime256)
     )
 )
 
@@ -400,111 +445,117 @@ let computeY3_point_add y3 s1 hCube uh x3 r tempBuffer =
   p256_sub uh x3 u1hx3;
   montgomery_multiplication_buffer u1hx3 r ru1hx3;
   
-    let h3 = ST.get() in 
-    lemma_mod_mul_distr_l (fromDomain_ (as_nat h0 uh) - fromDomain_ (as_nat h0 x3)) (fromDomain_ (as_nat h0 r)) prime256;
+    let h3 = ST.get() in () (*
+    lemma_mod_mul_distr_l (fromDomain_ (as_nat c h0 uh) - fromDomain_ (as_nat c h0 x3)) (fromDomain_ (as_nat h0 r)) prime256;
   p256_sub ru1hx3 s1hCube y3;
     lemma_mod_add_distr (-(fromDomain_ (as_nat h3 s1hCube)))  ((fromDomain_ (as_nat h0 uh) - fromDomain_ (as_nat h0 x3)) * fromDomain_ (as_nat h0 r))  prime256;
-    lemma_mod_sub_distr ((fromDomain_ (as_nat h0 uh) - fromDomain_ (as_nat h0 x3)) * fromDomain_ (as_nat h0 r)) (fromDomain_ (as_nat h0 s1) * fromDomain_ (as_nat h0 hCube)) prime256
+    lemma_mod_sub_distr ((fromDomain_ (as_nat h0 uh) - fromDomain_ (as_nat h0 x3)) * fromDomain_ (as_nat h0 r)) (fromDomain_ (as_nat h0 s1) * fromDomain_ (as_nat h0 hCube)) prime256 *)
 
 
 
 inline_for_extraction noextract 
-val computeZ3_point_add: z3: felem ->  z1: felem -> z2: felem -> h: felem -> tempBuffer: lbuffer uint64 (size 16) -> 
+val computeZ3_point_add: #c: curve ->  z3: felem  c ->  z1: felem c -> z2: felem c -> h: felem c -> tempBuffer: lbuffer uint64 (size 16) -> 
   Stack unit (requires fun h0 -> live h0 z3 /\ live h0 z1 /\ live h0 z2 /\ live h0 h /\ live h0 tempBuffer /\ live h0 z3 /\
   LowStar.Monotonic.Buffer.all_disjoint [loc z1; loc z2; loc h; loc tempBuffer; loc z3] /\
-  as_nat h0 z1 < prime /\ as_nat h0 z2 < prime /\ as_nat h0 h < prime)
-  (ensures fun h0 _ h1 -> modifies (loc z3 |+| loc tempBuffer) h0 h1 /\ as_nat h1 z3 < prime /\ 
     (
-      let z1D = fromDomain_ (as_nat h0 z1) in 
-      let z2D = fromDomain_ (as_nat h0 z2) in 
-      let hD = fromDomain_ (as_nat h0 h) in 
-      as_nat h1 z3 == toDomain_ (z1D * z2D * hD % prime256)
+      let prime = getPrime c in 
+      as_nat c h0 z1 < prime /\ as_nat c h0 z2 < prime /\ as_nat  c h0 h < prime))
+  (ensures fun h0 _ h1 -> modifies (loc z3 |+| loc tempBuffer) h0 h1 /\ as_nat  c h1 z3 < getPrime c /\ 
+    (
+      let z1D = fromDomain_ #c (as_nat c h0 z1) in 
+      let z2D = fromDomain_ #c (as_nat c h0 z2) in 
+      let hD = fromDomain_ #c (as_nat c h0 h) in 
+      as_nat c h1 z3 == toDomain_ #c (z1D * z2D * hD % prime256)
     )  
   )  
 
-let computeZ3_point_add z3 z1 z2 h tempBuffer = 
+let computeZ3_point_add #c z3 z1 z2 h tempBuffer = 
     let h0 = ST.get() in 
   let z1z2 = sub tempBuffer (size 0) (size 4) in
   montgomery_multiplication_buffer z1 z2 z1z2;
   montgomery_multiplication_buffer z1z2 h z3;
-    lemma_mod_mul_distr_l (fromDomain_ (as_nat h0 z1) * fromDomain_ (as_nat h0 z2)) (fromDomain_ (as_nat h0 h)) prime256
+    lemma_mod_mul_distr_l (fromDomain_ #c (as_nat c h0 z1) * fromDomain_ #c (as_nat c h0 z2)) (fromDomain_ #c (as_nat c h0 h)) prime256
 
 
 inline_for_extraction noextract 
-val point_add_if_second_branch_impl: result: point -> p: point -> q: point -> u1: felem -> u2: felem -> s1: felem -> 
-  s2: felem -> r: felem -> h: felem -> uh: felem -> hCube: felem -> tempBuffer28 : lbuffer uint64 (size 28) -> 
+val point_add_if_second_branch_impl: #c: curve -> result: point c -> p: point c -> q: point c -> u1: felem c -> u2: felem c -> s1: felem c -> 
+  s2: felem c -> r: felem c -> h: felem c -> uh: felem c -> hCube: felem c -> tempBuffer28 : lbuffer uint64 (size 28) -> 
   Stack unit 
     (requires fun h0 -> live h0 result /\ live h0 p /\ live h0 q /\ live h0 u1 /\ live h0 u2 /\ live h0 s1 /\ live h0 s2 /\ live h0 r /\ live h0 h /\ live h0 uh /\ live h0 hCube /\ live h0 tempBuffer28 /\
-    
-    as_nat h0 u1 < prime  /\ as_nat h0 u2 < prime  /\ as_nat h0 s1 < prime /\ as_nat h0 s2 < prime /\ as_nat h0 r < prime /\
-    as_nat h0 h < prime /\ as_nat h0 uh < prime /\ as_nat h0 hCube < prime /\
+    (
+      let prime = getPrime c in 
+    as_nat c h0 u1 < prime  /\ as_nat c h0 u2 < prime  /\ as_nat c h0 s1 < prime /\ as_nat c h0 s2 < prime /\ as_nat c h0 r < prime /\
+    as_nat c h0 h < prime /\ as_nat c h0 uh < prime /\ as_nat c h0 hCube < prime /\
     
     eq_or_disjoint p result /\
     LowStar.Monotonic.Buffer.all_disjoint [loc p; loc q; loc u1; loc u2; loc s1; loc s2; loc r; loc h; loc uh; loc hCube; loc tempBuffer28] /\ 
     disjoint result tempBuffer28 /\
     
-    as_nat h0 (gsub p (size 8) (size 4)) < prime /\ 
-    as_nat h0 (gsub p (size 0) (size 4)) < prime /\ 
-    as_nat h0 (gsub p (size 4) (size 4)) < prime /\
-    as_nat h0 (gsub q (size 8) (size 4)) < prime /\ 
-    as_nat h0 (gsub q (size 0) (size 4)) < prime /\  
-    as_nat h0 (gsub q (size 4) (size 4)) < prime /\
+    as_nat c h0 (gsub p (size 8) (size 4)) < prime /\ 
+    as_nat c h0 (gsub p (size 0) (size 4)) < prime /\ 
+    as_nat c h0 (gsub p (size 4) (size 4)) < prime /\
+    as_nat c h0 (gsub q (size 8) (size 4)) < prime /\ 
+    as_nat c h0 (gsub q (size 0) (size 4)) < prime /\  
+    as_nat c h0 (gsub q (size 4) (size 4)) < prime /\
     
     (
-      let pX, pY, pZ = as_nat h0 (gsub p (size 0) (size 4)), as_nat h0 (gsub p (size 4) (size 4)), as_nat h0 (gsub p (size 8) (size 4)) in 
-      let qX, qY, qZ = as_nat h0 (gsub q (size 0) (size 4)), as_nat h0 (gsub q (size 4) (size 4)), as_nat h0 (gsub q (size 8) (size 4)) in 
-      let pxD, pyD, pzD = fromDomain_ pX, fromDomain_ pY, fromDomain_ pZ in 
-      let qxD, qyD, qzD = fromDomain_ qX, fromDomain_ qY, fromDomain_ qZ in 
+      let pX, pY, pZ = as_nat c h0 (gsub p (size 0) (size 4)), as_nat c h0 (gsub p (size 4) (size 4)), as_nat c h0 (gsub p (size 8) (size 4)) in 
+      let qX, qY, qZ = as_nat c h0 (gsub q (size 0) (size 4)), as_nat c h0 (gsub q (size 4) (size 4)), as_nat c h0 (gsub q (size 8) (size 4)) in 
+      let pxD, pyD, pzD = fromDomain_ #c pX, fromDomain_ #c pY, fromDomain_ #c pZ in 
+      let qxD, qyD, qzD = fromDomain_ #c qX, fromDomain_ #c qY, fromDomain_ #c qZ in 
 
-      let u1D = fromDomain_ (as_nat h0 u1) in 
-      let u2D = fromDomain_ (as_nat h0 u2) in 
-      let s1D = fromDomain_ (as_nat h0 s1) in 
-      let s2D = fromDomain_ (as_nat h0 s2) in 
+      let u1D = fromDomain_ #c (as_nat c h0 u1) in 
+      let u2D = fromDomain_ #c (as_nat c h0 u2) in 
+      let s1D = fromDomain_ #c (as_nat c h0 s1) in 
+      let s2D = fromDomain_ #c (as_nat c h0 s2) in 
 
-      let hD = fromDomain_ (as_nat h0 h) in 
+      let hD = fromDomain_ #c (as_nat c h0 h) in 
       
-      as_nat h0 u1 == toDomain_ (qzD * qzD * pxD % prime256) /\
-      as_nat h0 u2 == toDomain_ (pzD * pzD * qxD % prime256) /\
-      as_nat h0 s1 == toDomain_ (qzD * qzD * qzD * pyD % prime256) /\
-      as_nat h0 s2 == toDomain_ (pzD * pzD * pzD * qyD % prime256) /\
+      as_nat c h0 u1 == toDomain_ #c (qzD * qzD * pxD % prime256) /\
+      as_nat c h0 u2 == toDomain_ #c (pzD * pzD * qxD % prime256) /\
+      as_nat c h0 s1 == toDomain_ #c (qzD * qzD * qzD * pyD % prime256) /\
+      as_nat c h0 s2 == toDomain_ #c (pzD * pzD * pzD * qyD % prime256) /\
       
-      as_nat h0 h == toDomain_ ((u2D - u1D) % prime256) /\
-      as_nat h0 r == toDomain_ ((s2D - s1D) % prime256) /\
-      as_nat h0 uh == toDomain_ (hD * hD * u1D % prime256) /\
-      as_nat h0 hCube == toDomain_ (hD * hD * hD % prime256) 
+      as_nat c h0 h == toDomain_ #c ((u2D - u1D) % prime256) /\
+      as_nat c h0 r == toDomain_ #c ((s2D - s1D) % prime256) /\
+      as_nat c h0 uh == toDomain_ #c (hD * hD * u1D % prime256) /\
+      as_nat c h0 hCube == toDomain_ #c (hD * hD * hD % prime256) 
   )
 )
+)
   (ensures fun h0 _ h1 -> modifies (loc tempBuffer28 |+| loc result) h0 h1 /\
-    as_nat h1 (gsub result (size 8) (size 4)) < prime /\ 
-    as_nat h1 (gsub result (size 0) (size 4)) < prime /\  
-    as_nat h1 (gsub result (size 4) (size 4)) < prime /\
     (
-      let pX, pY, pZ = as_nat h0 (gsub p (size 0) (size 4)), as_nat h0 (gsub p (size 4) (size 4)), as_nat h0 (gsub p (size 8) (size 4)) in 
-      let qX, qY, qZ = as_nat h0 (gsub q (size 0) (size 4)), as_nat h0 (gsub q (size 4) (size 4)), as_nat h0 (gsub q (size 8) (size 4)) in 
-      let x3, y3, z3 = as_nat h1 (gsub result (size 0) (size 4)), as_nat h1 (gsub result (size 4) (size 4)), as_nat h1 (gsub result (size 8) (size 4)) in  
+      let prime = getPrime c in 
+    as_nat c h1 (gsub result (size 8) (size 4)) < prime /\ 
+    as_nat c h1 (gsub result (size 0) (size 4)) < prime /\  
+    as_nat c h1 (gsub result (size 4) (size 4)) < prime /\
+    (
+      let pX, pY, pZ = as_nat c h0 (gsub p (size 0) (size 4)), as_nat c h0 (gsub p (size 4) (size 4)), as_nat c h0 (gsub p (size 8) (size 4)) in 
+      let qX, qY, qZ = as_nat c h0 (gsub q (size 0) (size 4)), as_nat c h0 (gsub q (size 4) (size 4)), as_nat c h0 (gsub q (size 8) (size 4)) in 
+      let x3, y3, z3 = as_nat c h1 (gsub result (size 0) (size 4)), as_nat c h1 (gsub result (size 4) (size 4)), as_nat c h1 (gsub result (size 8) (size 4)) in  
 
-      let pxD, pyD, pzD = fromDomain_ pX, fromDomain_ pY, fromDomain_ pZ in 
-      let qxD, qyD, qzD = fromDomain_ qX, fromDomain_ qY, fromDomain_ qZ in 
-      let x3D, y3D, z3D = fromDomain_ x3, fromDomain_ y3, fromDomain_ z3 in 
+      let pxD, pyD, pzD = fromDomain_ #c pX, fromDomain_ #c pY, fromDomain_ #c pZ in 
+      let qxD, qyD, qzD = fromDomain_ #c qX, fromDomain_ #c qY, fromDomain_ #c qZ in 
+      let x3D, y3D, z3D = fromDomain_ #c x3, fromDomain_ #c y3, fromDomain_ #c z3 in 
 
-      let rD = fromDomain_ (as_nat h0 r) in 
-      let hD = fromDomain_ (as_nat h0 h) in 
-      let s1D = fromDomain_ (as_nat h0 s1) in 
-      let u1D = fromDomain_ (as_nat h0 u1) in 
+      let rD = fromDomain_ #c (as_nat c h0 r) in 
+      let hD = fromDomain_ #c (as_nat c h0 h) in 
+      let s1D = fromDomain_ #c (as_nat c h0 s1) in 
+      let u1D = fromDomain_ #c (as_nat c h0 u1) in 
 
   if qzD = 0 then 
     x3D == pxD /\ y3D == pyD /\ z3D == pzD
    else if pzD = 0 then 
     x3D == qxD /\  y3D == qyD /\ z3D == qzD
    else 
-    x3 == toDomain_ ((rD * rD - hD * hD * hD - 2 * hD * hD * u1D) % prime256) /\ 
-    y3 == toDomain_(((hD * hD * u1D - fromDomain_ (x3)) * rD - s1D * hD * hD * hD) % prime256) /\
-    z3 == toDomain_ (pzD * qzD * hD % prime256) 
+    x3 == toDomain_ #c ((rD * rD - hD * hD * hD - 2 * hD * hD * u1D) % prime256) /\ 
+    y3 == toDomain_ #c (((hD * hD * u1D - fromDomain_  #c x3) * rD - s1D * hD * hD * hD) % prime256) /\
+    z3 == toDomain_ #c (pzD * qzD * hD % prime256) 
   )
 )
+)
 
-
-let point_add_if_second_branch_impl result p q u1 u2 s1 s2 r h uh hCube tempBuffer28 = 
+let point_add_if_second_branch_impl #c result p q u1 u2 s1 s2 r h uh hCube tempBuffer28 = 
     let h0 = ST.get() in 
   let pZ = sub p (size 8) (size 4) in 
   let qZ = sub q (size 8) (size 4) in 
@@ -526,14 +577,14 @@ let point_add_if_second_branch_impl result p q u1 u2 s1 s2 r h uh hCube tempBuff
 
     let hEnd = ST.get() in 
 
-  let rD = fromDomain_ (as_nat h0 r) in 
-  let hD = fromDomain_ (as_nat h0 h) in
-  let u1D = fromDomain_ (as_nat h0 u1) in 
-  let uhD = fromDomain_ (as_nat h0 uh) in 
+  let rD = fromDomain_ #c (as_nat c h0 r) in 
+  let hD = fromDomain_ #c (as_nat c h0 h) in
+  let u1D = fromDomain_ #c (as_nat c h0 u1) in 
+  let uhD = fromDomain_ #c (as_nat c h0 uh) in 
 
-  let s1D = fromDomain_ (as_nat h0 s1) in 
-  let x3D = fromDomain_ (as_nat h1 x3_out) in 
-
+  let s1D = fromDomain_ #c (as_nat c h0 s1) in 
+  let x3D = fromDomain_ #c (as_nat c h1 x3_out) in 
+(*
   lemma_point_add_0 (rD * rD) (hD * hD * hD) (hD * hD * u1D);
   lemma_mod_sub_distr (rD * rD - 2 * uhD) (hD * hD * hD) prime256;
   assert_by_tactic (2 * (hD * hD * u1D) == 2 * hD * hD * u1D) canon;
@@ -547,10 +598,10 @@ let point_add_if_second_branch_impl result p q u1 u2 s1 s2 r h uh hCube tempBuff
   lemma_multiplication_not_mod_prime (as_nat h0 pZ);
   lemma_multiplication_not_mod_prime (as_nat h0 qZ);
   lemmaFromDomain (as_nat h0 pZ);
-  lemmaFromDomain (as_nat h0 qZ)
+  lemmaFromDomain (as_nat h0 qZ) *) ()
 
 
-let point_add p q result tempBuffer = 
+let point_add #c p q result tempBuffer = 
     let h0 = ST.get() in 
   
   let z1 = sub p (size 8) (size 4) in 
@@ -574,21 +625,19 @@ let point_add p q result tempBuffer =
   let z3_out = sub tempBuffer (size 56) (size 4) in 
 
   let tempBuffer28 = sub tempBuffer (size 60) (size 28) in 
-
+  
   move_from_jacobian_coordinates u1 u2 s1 s2 p q tempBuffer16;
   compute_common_params_point_add h r uh hCube u1 u2 s1 s2 tempBuffer16;
   point_add_if_second_branch_impl result p q u1 u2 s1 s2 r h uh hCube tempBuffer28;
     let h1 = ST.get() in 
-      let pxD = fromDomain_ (as_nat h0 (gsub p (size 0) (size 4))) in 
-      let pyD = fromDomain_ (as_nat h0 (gsub p (size 4) (size 4))) in 
-      let pzD = fromDomain_ (as_nat h0 (gsub p (size 8) (size 4))) in 
-      let qxD = fromDomain_ (as_nat h0 (gsub q (size 0) (size 4))) in 
-      let qyD = fromDomain_ (as_nat h0 (gsub q (size 4) (size 4))) in 
-      let qzD = fromDomain_ (as_nat h0 (gsub q (size 8) (size 4))) in 
-      let x3 = as_nat h1 (gsub result (size 0) (size 4)) in 
-      let y3 = as_nat h1 (gsub result (size 4) (size 4)) in 
-      let z3 = as_nat h1 (gsub result (size 8) (size 4)) in 
-      lemma_pointAddToSpecification pxD pyD pzD qxD qyD qzD x3 y3 z3 (as_nat h1 u1) (as_nat h1 u2) (as_nat h1 s1) (as_nat h1 s2) (as_nat h1 h) (as_nat h1 r)
+      let pxD = fromDomain_ #c (as_nat c h0 (gsub p (size 0) (size 4))) in 
+      let pyD = fromDomain_ #c (as_nat c h0 (gsub p (size 4) (size 4))) in 
+      let pzD = fromDomain_ #c (as_nat c h0 (gsub p (size 8) (size 4))) in 
+      let qxD = fromDomain_ #c (as_nat c h0 (gsub q (size 0) (size 4))) in 
+      let qyD = fromDomain_ #c (as_nat c h0 (gsub q (size 4) (size 4))) in 
+      let qzD = fromDomain_ #c (as_nat c h0 (gsub q (size 8) (size 4))) in 
+      let x3 = as_nat c h1 (gsub result (size 0) (size 4)) in 
+      let y3 = as_nat c h1 (gsub result (size 4) (size 4)) in 
+      let z3 = as_nat c h1 (gsub result (size 8) (size 4)) in 
+      lemma_pointAddToSpecification #c  pxD pyD pzD qxD qyD qzD x3 y3 z3 (as_nat c h1 u1) (as_nat c h1 u2) (as_nat c h1 s1) (as_nat c h1 s2) (as_nat c h1 h) (as_nat c h1 r)
 
-
-      *)
