code/ecdsap256/Hacl.Impl.P256.PointDouble.fst
@@ -307,13 +307,13 @@ val point_double_a_b_g: #c: curve
       (
 	let coordinateLen = getCoordinateLenU64 c in 
 	let prime = getPrime c in 
-	let x = fromDomain_ (as_nat c h0 (gsub p (size 0) (size coordinateLen))) in 
-	let y = fromDomain_ (as_nat c h0 (gsub p (size coordinateLen) (size coordinateLen))) in 
-	let z = fromDomain_ (as_nat c h0 (gsub p (size (2 * coordinateLen)) (size coordinateLen))) in 
-	as_nat c h1 delta = toDomain_ (z * z % prime) /\
-	as_nat c h1 gamma = toDomain_ (y * y % prime) /\
-	as_nat c h1 beta = toDomain_ (x * fromDomain_ (as_nat c h1 gamma) % prime) /\
-	as_nat c h1 alpha = toDomain_ (3 * (x - fromDomain_ (as_nat c h1 delta)) * (x + fromDomain_ (as_nat c h1 delta)) % prime)
+	let x = fromDomain_ #c (as_nat c h0 (gsub p (size 0) (size coordinateLen))) in 
+	let y = fromDomain_ #c (as_nat c h0 (gsub p (size coordinateLen) (size coordinateLen))) in 
+	let z = fromDomain_ #c (as_nat c h0 (gsub p (size (2 * coordinateLen)) (size coordinateLen))) in 
+	as_nat c h1 delta = toDomain_ #c (z * z % prime) /\
+	as_nat c h1 gamma = toDomain_ #c (y * y % prime) /\
+	as_nat c h1 beta = toDomain_ #c (x * fromDomain_ #c (as_nat c h1 gamma) % prime) /\
+	as_nat c h1 alpha = toDomain_ #c (3 * (x - fromDomain_ #c (as_nat c h1 delta)) * (x + fromDomain_ #c (as_nat c h1 delta)) % prime)
       )
     )
 
@@ -344,8 +344,8 @@ let point_double_a_b_g #c p alpha beta gamma delta tempBuffer =
 
     let prime = getPrime c in 
     let open FStar.Tactics.Canon in 
-    let xD = fromDomain_ (as_nat c h0 pX) in 
-    let dlt = fromDomain_ (as_nat c h0 delta) in 
+    let xD = fromDomain_ #c (as_nat c h0 pX) in 
+    let dlt = fromDomain_ #c (as_nat c h0 delta) in 
 
     calc (==) 
     {
@@ -370,8 +370,8 @@ val point_double_x3: #c: curve -> x3: felem c -> alpha: felem c -> fourBeta: fel
     (ensures fun h0 _ h1 -> modifies (loc x3 |+| loc fourBeta |+| loc eightBeta) h0 h1 /\
       (
 	let prime = getPrime c in 
-	as_nat c h1 fourBeta = toDomain_ (4 * fromDomain_ (as_nat c h0 beta) % getPrime c) /\
-	as_nat c h1 x3 = toDomain_ ((fromDomain_ (as_nat c h0 alpha) * fromDomain_ (as_nat c h0 alpha) - 8 * (fromDomain_ (as_nat c h0 beta))) % prime)
+	as_nat c h1 fourBeta = toDomain_ #c (4 * fromDomain_ #c (as_nat c h0 beta) % getPrime c) /\
+	as_nat c h1 x3 = toDomain_ #c ((fromDomain_ #c (as_nat c h0 alpha) * fromDomain_ #c (as_nat c h0 alpha) - 8 * (fromDomain_ #c (as_nat c h0 beta))) % prime)
       )
    ) 
 
@@ -386,19 +386,19 @@ let point_double_x3 #c x3 alpha fourBeta beta eightBeta  =
   let prime = getPrime c in 
   calc(==)
   {
-     toDomain_ (((fromDomain_ (as_nat c h0 alpha) * fromDomain_ (as_nat c h0 alpha) % prime) - (2 *  (4 * fromDomain_ (as_nat c h0 beta) % prime) % prime)) % prime);
+     toDomain_ #c (((fromDomain_ #c (as_nat c h0 alpha) * fromDomain_ #c (as_nat c h0 alpha) % prime) - (2 *  (4 * fromDomain_ #c (as_nat c h0 beta) % prime) % prime)) % prime);
      
-     (==) {lemma_mod_mul_distr_r 2 (4 * fromDomain_ (as_nat c h0 beta)) prime}
+     (==) {lemma_mod_mul_distr_r 2 (4 * fromDomain_ #c (as_nat c h0 beta)) prime}
   
-     toDomain_ (((fromDomain_ (as_nat c h0 alpha) * fromDomain_ (as_nat c h0 alpha) % prime) - (8 * fromDomain_ (as_nat c h0 beta)) % prime) % prime);
+     toDomain_ #c (((fromDomain_ #c (as_nat c h0 alpha) * fromDomain_ #c (as_nat c h0 alpha) % prime) - (8 * fromDomain_ #c (as_nat c h0 beta)) % prime) % prime);
      
-     (==) {lemma_mod_sub_distr (fromDomain_ (as_nat c h0 alpha) * fromDomain_ (as_nat c h0 alpha) % prime) (8 * fromDomain_ (as_nat c h0 beta)) prime}
+     (==) {lemma_mod_sub_distr (fromDomain_ #c (as_nat c h0 alpha) * fromDomain_ #c (as_nat c h0 alpha) % prime) (8 * fromDomain_ #c (as_nat c h0 beta)) prime}
      
-    toDomain_ (((fromDomain_ (as_nat c h0 alpha) * fromDomain_ (as_nat c h0 alpha) % prime) - (8 * fromDomain_ (as_nat c h0 beta))) % prime256);
+    toDomain_ #c (((fromDomain_ #c (as_nat c h0 alpha) * fromDomain_ #c (as_nat c h0 alpha) % prime) - (8 * fromDomain_ #c (as_nat c h0 beta))) % prime256);
  
-    (==) {lemma_mod_add_distr (- 8 * fromDomain_ (as_nat c h0 beta)) (fromDomain_ (as_nat c h0 alpha) * fromDomain_ (as_nat c h0 alpha)) prime}
+    (==) {lemma_mod_add_distr (- 8 * fromDomain_ #c (as_nat c h0 beta)) (fromDomain_ #c (as_nat c h0 alpha) * fromDomain_ #c (as_nat c h0 alpha)) prime}
       
-    toDomain_ ((fromDomain_ (as_nat c h0 alpha) * fromDomain_ (as_nat c h0 alpha) - 8 * fromDomain_ (as_nat c h0 beta)) % prime256);
+    toDomain_ #c ((fromDomain_ #c (as_nat c h0 alpha) * fromDomain_ #c (as_nat c h0 alpha) - 8 * fromDomain_ #c (as_nat c h0 beta)) % prime256);
   }
 
 
@@ -417,14 +417,15 @@ val point_double_z3: #c: curve -> z3: felem c -> pY: felem c -> pZ: felem c -> g
     (ensures fun h0 _ h1 -> modifies (loc z3) h0 h1 /\
       (
 	let prime = getPrime c in 
-	let y = fromDomain_ (as_nat c h0 pY) in 
-	let z = fromDomain_ (as_nat c h0 pZ) in 
-	as_nat c h1 z3 = toDomain_ (((y + z) * (y + z) - fromDomain_ (as_nat c h0 gamma) - fromDomain_ (as_nat c h0 delta)) % prime)
+	let y = fromDomain_ #c (as_nat c h0 pY) in 
+	let z = fromDomain_ #c (as_nat c h0 pZ) in 
+	as_nat c h1 z3 = toDomain_ #c (((y + z) * (y + z) - fromDomain_ #c (as_nat c h0 gamma) - fromDomain_ #c (as_nat c h0 delta)) % prime)
       )
     )
 
 let point_double_z3 #c z3 pY pZ gamma delta  = 
     let h0 = ST.get() in 
+  let prime = getPrime c in 
 
   felem_add pY pZ z3; (* z3 = py + pz *) 
   montgomery_square_buffer z3 z3; (* z3 = (py + pz) ** 2 *) 
@@ -432,24 +433,25 @@ let point_double_z3 #c z3 pY pZ gamma delta  =
   felem_sub z3 delta z3 (* z3 = (py + pz) ** 2 - gamma - delta *);
 
   admit();
-    let pyD = fromDomain_ (as_nat c h0 pY) in 
-    let pzD = fromDomain_ (as_nat c h0 pZ) in 
+    let pyD = fromDomain_ #c (as_nat c h0 pY) in 
+    let pzD = fromDomain_ #c (as_nat c h0 pZ) in 
 
   calc (==)
   {
-    toDomain_ (((((( ((pyD + pzD) % prime) * ((pyD + pzD) % prime) % prime)) - fromDomain_ (as_nat c h0 gamma)) % prime) - fromDomain_ (as_nat c h0 delta)) % prime);
+    toDomain_ #c (((((( ((pyD + pzD) % prime) * ((pyD + pzD) % prime) % prime)) - fromDomain_ #c (as_nat c h0 gamma)) % prime) - fromDomain_ #c (as_nat c h0 delta)) % prime);
   
-    (==) {lemma_mod_mul_distr_l (pyD + pzD) ((pyD + pzD) % prime) prime; lemma_mod_mul_distr_r (pyD + pzD) (pyD + pzD) prime}
+    (==) {lemma_mod_mul_distr_l (pyD + pzD) ((pyD + pzD) % prime) prime; 
+      lemma_mod_mul_distr_r (pyD + pzD) (pyD + pzD) prime}
     
-    toDomain_ ((((((pyD + pzD) * (pyD + pzD) % prime) - fromDomain_ (as_nat c h0 gamma)) % prime) - fromDomain_ (as_nat c h0 delta)) % prime);
+    toDomain_ #c ((((((pyD + pzD) * (pyD + pzD) % prime) - fromDomain_ #c (as_nat c h0 gamma)) % prime) - fromDomain_ #c (as_nat c h0 delta)) % prime);
     
-  (==) {lemma_mod_add_distr (- fromDomain_ (as_nat c h0 gamma)) ((pyD + pzD) * (pyD + pzD)) prime }
+  (==) {lemma_mod_add_distr (- fromDomain_ #c (as_nat c h0 gamma)) ((pyD + pzD) * (pyD + pzD)) prime }
     
-    toDomain_ (((((pyD + pzD) * (pyD + pzD) - fromDomain_ (as_nat c h0 gamma)) % prime) - fromDomain_ (as_nat c h0 delta)) % prime);
+    toDomain_ #c (((((pyD + pzD) * (pyD + pzD) - fromDomain_ #c (as_nat c h0 gamma)) % prime) - fromDomain_ #c (as_nat c h0 delta)) % prime);
  
-    (==) {lemma_mod_add_distr (- fromDomain_ (as_nat c h0 delta)) ((pyD + pzD) * (pyD + pzD) - fromDomain_ (as_nat c h0 gamma)) prime}
+    (==) {lemma_mod_add_distr (- fromDomain_ #c (as_nat c h0 delta)) ((pyD + pzD) * (pyD + pzD) - fromDomain_ #c (as_nat c h0 gamma)) prime}
     
-    toDomain_ (((pyD + pzD) * (pyD + pzD) - fromDomain_ (as_nat c h0 gamma) - fromDomain_ (as_nat c h0 delta)) % prime);
+    toDomain_ #c (((pyD + pzD) * (pyD + pzD) - fromDomain_ #c (as_nat c h0 gamma) - fromDomain_ #c (as_nat c h0 delta)) % prime);
   }
 
 
@@ -467,9 +469,9 @@ val point_double_y3: #c: curve -> y3: felem c -> x3: felem c -> alpha: felem c -
   )
   (ensures fun h0 _ h1 -> modifies (loc y3 |+| loc gamma |+| loc eightGamma) h0 h1 /\
     (
-      let alphaD = fromDomain_ (as_nat c h0 alpha) in 
-      let gammaD = fromDomain_ (as_nat c h0 gamma) in 
-      as_nat c h1 y3 == toDomain_ ((alphaD *  (fromDomain_ (as_nat c h0 fourBeta) - fromDomain_ (as_nat c h0 x3)) - 8 * gammaD * gammaD) % getPrime c)
+      let alphaD = fromDomain_ #c (as_nat c h0 alpha) in 
+      let gammaD = fromDomain_ #c (as_nat c h0 gamma) in 
+      as_nat c h1 y3 == toDomain_ #c ((alphaD *  (fromDomain_ #c (as_nat c h0 fourBeta) - fromDomain_ #c (as_nat c h0 x3)) - 8 * gammaD * gammaD) % getPrime c)
     )
   )
 
@@ -484,8 +486,8 @@ let point_double_y3 #c y3 x3 alpha gamma eightGamma fourBeta =
   p256_sub y3 eightGamma y3; (* y3 = alpha * y3 - 8 * gamma **2 *)
 
 
-  let alphaD = fromDomain_ (as_nat c h0 alpha) in 
-  let gammaD = fromDomain_ (as_nat c h0 gamma) in  
+  let alphaD = fromDomain_ #c (as_nat c h0 alpha) in 
+  let gammaD = fromDomain_ #c (as_nat c h0 gamma) in  
   admit();
 
   let open FStar.Tactics.Canon in 
@@ -494,49 +496,49 @@ let point_double_y3 #c y3 x3 alpha gamma eightGamma fourBeta =
 
   calc(==)
   {
-     toDomain_ (((fromDomain_ (as_nat c h0 alpha) *  ((fromDomain_ (as_nat c h0 fourBeta) - fromDomain_ (as_nat c h0 x3)) % prime) % prime) - (8 *  (fromDomain_ (as_nat c h0 gamma) * fromDomain_ (as_nat c h0 gamma) % prime) % prime)) % prime);
+     toDomain_ #c (((fromDomain_ #c (as_nat c h0 alpha) *  ((fromDomain_ #c (as_nat c h0 fourBeta) - fromDomain_ #c (as_nat c h0 x3)) % prime) % prime) - (8 *  (fromDomain_ #c (as_nat c h0 gamma) * fromDomain_ #c (as_nat c h0 gamma) % prime) % prime)) % prime);
  
-     (==) {lemma_mod_mul_distr_r (fromDomain_ (as_nat c h0 alpha)) (((fromDomain_ (as_nat c h0 fourBeta) - fromDomain_ (as_nat c h0 x3)))) prime}
+     (==) {lemma_mod_mul_distr_r (fromDomain_ #c (as_nat c h0 alpha)) (((fromDomain_ #c (as_nat c h0 fourBeta) - fromDomain_ #c (as_nat c h0 x3)))) prime}
     
-    toDomain_ (((fromDomain_ (as_nat c h0 alpha) *  (fromDomain_ (as_nat c h0 fourBeta) - fromDomain_ (as_nat c h0 x3)) % prime) - (8 *  (fromDomain_ (as_nat c h0 gamma) * fromDomain_ (as_nat c h0 gamma) % prime) % prime)) % prime);
+    toDomain_ #c (((fromDomain_ #c (as_nat c h0 alpha) *  (fromDomain_ #c (as_nat c h0 fourBeta) - fromDomain_ #c (as_nat c h0 x3)) % prime) - (8 *  (fromDomain_ #c (as_nat c h0 gamma) * fromDomain_ #c (as_nat c h0 gamma) % prime) % prime)) % prime);
     
-    (==) {lemma_mod_mul_distr_r 8 (fromDomain_ (as_nat c h0 gamma) * (fromDomain_ (as_nat c h0 gamma))) prime}
+    (==) {lemma_mod_mul_distr_r 8 (fromDomain_ #c (as_nat c h0 gamma) * (fromDomain_ #c (as_nat c h0 gamma))) prime}
     
-    toDomain_ (((alphaD *  (fromDomain_ (as_nat c h0 fourBeta) - fromDomain_ (as_nat c h0 x3)) % prime) - (8 * (gammaD * gammaD) % prime)) % prime);
+    toDomain_ #c (((alphaD *  (fromDomain_ #c (as_nat c h0 fourBeta) - fromDomain_ #c (as_nat c h0 x3)) % prime) - (8 * (gammaD * gammaD) % prime)) % prime);
   
-    (==) {lemma_mod_add_distr (-(8 * (gammaD * gammaD) % prime)) (alphaD *  (fromDomain_ (as_nat c h0 fourBeta) - fromDomain_ (as_nat c h0 x3))) prime  }
+    (==) {lemma_mod_add_distr (-(8 * (gammaD * gammaD) % prime)) (alphaD *  (fromDomain_ #c (as_nat c h0 fourBeta) - fromDomain_ #c (as_nat c h0 x3))) prime  }
     
-    toDomain_ (((alphaD *  (fromDomain_ (as_nat c h0 fourBeta) - fromDomain_ (as_nat c h0 x3))) - (8 * (gammaD * gammaD) % prime)) % prime);
+    toDomain_ #c (((alphaD *  (fromDomain_ #c (as_nat c h0 fourBeta) - fromDomain_ #c (as_nat c h0 x3))) - (8 * (gammaD * gammaD) % prime)) % prime);
     
-    (==) {lemma_mod_sub_distr (alphaD *  (fromDomain_ (as_nat c h0 fourBeta) - fromDomain_ (as_nat c h0 x3))) (8 * (gammaD * gammaD)) prime}
+    (==) {lemma_mod_sub_distr (alphaD *  (fromDomain_ #c (as_nat c h0 fourBeta) - fromDomain_ #c (as_nat c h0 x3))) (8 * (gammaD * gammaD)) prime}
     
-    toDomain_ (((alphaD *  (fromDomain_ (as_nat c h0 fourBeta) - fromDomain_ (as_nat c h0 x3))) - (8 * (gammaD * gammaD))) % prime);
+    toDomain_ #c (((alphaD *  (fromDomain_ #c (as_nat c h0 fourBeta) - fromDomain_ #c (as_nat c h0 x3))) - (8 * (gammaD * gammaD))) % prime);
     
     (==) {assert_by_tactic (8 * (gammaD * gammaD) == 8 * gammaD * gammaD) canon}
     
-    toDomain_ ((alphaD *  (fromDomain_ (as_nat c h0 fourBeta) - fromDomain_ (as_nat c h0 x3)) - 8 * gammaD * gammaD) % prime);
+    toDomain_ #c ((alphaD *  (fromDomain_ #c (as_nat c h0 fourBeta) - fromDomain_ #c (as_nat c h0 x3)) - 8 * gammaD * gammaD) % prime);
 }
 
 
 val lemma_pd_to_spec: #c: curve -> x: nat -> y: nat -> z: nat -> x3: nat -> y3: nat -> z3: nat ->  Lemma 
   (requires (  
     let prime = getPrime c in 
-    let xD, yD, zD = fromDomain_ x, fromDomain_ y, fromDomain_ z in 
-    x3 == toDomain_ (((3 * (xD - zD * zD) * (xD + zD * zD)) * (3 * (xD - zD * zD) * (xD + zD * zD)) - 8 * xD * (yD * yD)) % prime) /\
-    y3 == toDomain_ ((3 * (xD - zD * zD) * (xD + zD * zD) *  (4 * xD * (yD * yD) - fromDomain_ x3) - 8 * (yD * yD) * (yD * yD)) % prime) /\
-    z3 = toDomain_ (((yD + zD) * (yD + zD) - zD * zD - yD * yD) % prime)
+    let xD, yD, zD = fromDomain_ #c x, fromDomain_ #c y, fromDomain_ #c z in 
+    x3 == toDomain_ #c (((3 * (xD - zD * zD) * (xD + zD * zD)) * (3 * (xD - zD * zD) * (xD + zD * zD)) - 8 * xD * (yD * yD)) % prime) /\
+    y3 == toDomain_ #c ((3 * (xD - zD * zD) * (xD + zD * zD) *  (4 * xD * (yD * yD) - fromDomain_ #c x3) - 8 * (yD * yD) * (yD * yD)) % prime) /\
+    z3 = toDomain_ #c (((yD + zD) * (yD + zD) - zD * zD - yD * yD) % prime)
   )
 )
  (ensures(
-   let xD, yD, zD = fromDomain_ x, fromDomain_ y, fromDomain_ z in 
-   let x3D, y3D, z3D = fromDomain_ x3, fromDomain_ y3, fromDomain_ z3 in 
+   let xD, yD, zD = fromDomain_ #c x, fromDomain_ #c y, fromDomain_ #c z in 
+   let x3D, y3D, z3D = fromDomain_ #c x3, fromDomain_ #c y3, fromDomain_ #c z3 in 
    let xN, yN, zN = _point_double #c (xD, yD, zD) in 
    x3D == xN /\ y3D == yN /\ z3D == zN))
 
 
 let lemma_pd_to_spec #c x y z x3 y3 z3 = 
-  let xD, yD, zD = fromDomain_ x, fromDomain_ y, fromDomain_ z in 
-  let x3D, y3D, z3D = fromDomain_ x3, fromDomain_ y3, fromDomain_ z3 in 
+  let xD, yD, zD = fromDomain_ #c x, fromDomain_ #c y, fromDomain_ #c z in 
+  let x3D, y3D, z3D = fromDomain_ #c x3, fromDomain_ #c y3, fromDomain_ #c z3 in 
   assert(let xN, yN, zN = _point_double #c  (xD, yD, zD) in 
       x3D == xN /\ y3D == yN /\ z3D == zN)
 
@@ -573,13 +575,13 @@ let point_double #c p result tempBuffer =
 
   let h4 = ST.get() in
 
-  let x = fromDomain_ (as_nat c h0 (gsub p (size 0) (size len))) in 
-  let y = fromDomain_ (as_nat c h0 (gsub p (size len) (size len))) in 
-  let z = fromDomain_ (as_nat c h0 (gsub p (size (2 * len)) (size len))) in 
+  let x = fromDomain_ #c (as_nat c h0 (gsub p (size 0) (size len))) in 
+  let y = fromDomain_ #c (as_nat c h0 (gsub p (size len) (size len))) in 
+  let z = fromDomain_ #c (as_nat c h0 (gsub p (size (2 * len)) (size len))) in 
   
   lemma_x3 #c x y z;
   lemma_z3 #c x y z;
-  lemma_y3 #c x y z (fromDomain_ (as_nat c h4 x3));
+  lemma_y3 #c x y z (fromDomain_ #c (as_nat c h4 x3));
   lemma_pd_to_spec #c
     (as_nat c h0 (gsub p (size 0) (size len))) 
       (as_nat c h0 (gsub p (size len) (size len))) 
