code/ecdsap256/Hacl.Impl.P256.Arithmetics.fsti
@@ -26,47 +26,47 @@ val cube: #c: curve -> a: felem c -> result: felem c -> Stack unit
   (requires fun h -> live h a /\ live h result /\ disjoint a result /\ as_nat c h a < getPrime c)
   (ensures fun h0 _ h1 -> modifies (loc result) h0 h1 /\ 
     as_nat c h1 result < getPrime c /\
-    as_nat c h1 result = toDomain_ (fromDomain_ (as_nat c h0 a) * fromDomain_ (as_nat c h0 a) * fromDomain_ (as_nat c h0 a) % getPrime c) /\ 
-    as_nat c h1 result = toDomain_ (fromDomain_ (as_nat c h0 a) * fromDomain_ (as_nat c h0 a) * fromDomain_ (as_nat c h0 a)))
+    as_nat c h1 result = toDomain_ #c (fromDomain_ #c (as_nat c h0 a) * fromDomain_ #c (as_nat c h0 a) * fromDomain_ #c (as_nat c h0 a) % getPrime c) /\ 
+    as_nat c h1 result = toDomain_ #c (fromDomain_ #c (as_nat c h0 a) * fromDomain_ #c (as_nat c h0 a) * fromDomain_ #c (as_nat c h0 a)))
 
 
 inline_for_extraction noextract
 val quatre: #c: curve -> a: felem c -> result: felem c -> Stack unit
   (requires fun h -> live h a /\ live h result /\ disjoint a result /\ as_nat c h a < getPrime c)
   (ensures fun h0 _ h1 -> modifies (loc result) h0 h1 /\ 
-    as_nat c h1 result = toDomain_ (fromDomain_ (as_nat c h0 a) * fromDomain_ (as_nat c h0 a) * fromDomain_ (as_nat c h0 a) * fromDomain_ (as_nat c h0 a) % getPrime c) /\ 
-    as_nat c h1 result = toDomain_ (fromDomain_ (as_nat c h0 a) * fromDomain_ (as_nat c h0 a) * fromDomain_ (as_nat c h0 a) * fromDomain_ (as_nat c h0 a)))
+    as_nat c h1 result = toDomain_ #c (fromDomain_ #c (as_nat c h0 a) * fromDomain_ #c (as_nat c h0 a) * fromDomain_ #c (as_nat c h0 a) * fromDomain_ #c (as_nat c h0 a) % getPrime c) /\ 
+    as_nat c h1 result = toDomain_ #c (fromDomain_ #c (as_nat c h0 a) * fromDomain_ #c (as_nat c h0 a) * fromDomain_ #c (as_nat c h0 a) * fromDomain_ #c (as_nat c h0 a)))
 
 
 val multByTwo: #c: curve -> a: felem c -> result: felem c -> Stack unit 
   (requires fun h -> live h a /\ live h result /\ eq_or_disjoint a result /\ as_nat c h a < getPrime c)
   (ensures fun h0 _ h1 -> modifies (loc result) h0 h1 /\ 
-    as_nat c h1 result == toDomain_ (2 * fromDomain_ (as_nat c h0 a) % getPrime c) /\ 
-    as_nat c h1 result == toDomain_ (2 * fromDomain_ (as_nat c h0 a)) /\ 
+    as_nat c h1 result == toDomain_ #c (2 * fromDomain_ #c (as_nat c h0 a) % getPrime c) /\ 
+    as_nat c h1 result == toDomain_ #c (2 * fromDomain_ #c (as_nat c h0 a)) /\ 
     as_nat c h1 result < getPrime c)
 
 
 val multByThree: #c: curve -> a: felem c -> result: felem c -> Stack unit 
   (requires fun h -> live h a /\ live h result /\ disjoint a result /\ as_nat c h a < getPrime c)
   (ensures fun h0 _ h1 -> modifies (loc result) h0 h1 /\ as_nat c h1 result < getPrime c /\ 
-    as_nat c h1 result == toDomain_ (3 * fromDomain_ (as_nat c h0 a) % getPrime c) /\ 
-    as_nat c h1 result == toDomain_ (3 * fromDomain_ (as_nat c h0 a))
+    as_nat c h1 result == toDomain_ #c (3 * fromDomain_ #c (as_nat c h0 a) % getPrime c) /\ 
+    as_nat c h1 result == toDomain_ #c (3 * fromDomain_ #c (as_nat c h0 a))
   )
 
 
 val multByFour: #c: curve -> a: felem c -> result: felem c -> Stack unit 
   (requires fun h -> live h a /\ live h result /\ eq_or_disjoint a result /\ as_nat c h a < getPrime c)
   (ensures fun h0 _ h1 -> modifies (loc result) h0 h1 /\ as_nat c h1 result < getPrime c /\ 
-    as_nat c h1 result == toDomain_ (4 * fromDomain_ (as_nat c h0 a) % getPrime c) /\ 
-    as_nat c h1 result == toDomain_ (4 * fromDomain_ (as_nat c h0 a))
+    as_nat c h1 result == toDomain_ #c (4 * fromDomain_ #c (as_nat c h0 a) % getPrime c) /\ 
+    as_nat c h1 result == toDomain_ #c (4 * fromDomain_ #c (as_nat c h0 a))
 )
 
 
 val multByEight: #c: curve -> a: felem c -> result: felem c -> Stack unit 
   (requires fun h -> live h a /\ live h result /\ disjoint a result /\ as_nat c h a < getPrime c)
   (ensures fun h0 _ h1 -> modifies (loc result) h0 h1 /\ as_nat c h1 result < getPrime c /\ 
-    as_nat c h1 result == toDomain_ (8 * fromDomain_ (as_nat c h0 a) % getPrime c) /\ 
-    as_nat c h1 result == toDomain_ (8 * fromDomain_ (as_nat c h0 a))
+    as_nat c h1 result == toDomain_ #c (8 * fromDomain_ #c (as_nat c h0 a) % getPrime c) /\ 
+    as_nat c h1 result == toDomain_ #c (8 * fromDomain_ #c (as_nat c h0 a))
 )
 
 
@@ -74,5 +74,5 @@ val multByMinusThree: #c: curve -> a: felem c -> result: felem c -> Stack unit
   (requires fun h -> live h a /\ live h result /\ disjoint a result /\ as_nat c h a < getPrime c)
   (ensures fun h0 _ h1 -> modifies (loc result) h0 h1 /\ 
     as_nat c h1 result < getPrime c /\ 
-    as_nat c h1 result == toDomain_ ((-3) * fromDomain_ (as_nat c h0 a) % getPrime c) /\
-    as_nat c h1 result == toDomain_ ((-3) * fromDomain_ (as_nat c h0 a)))
+    as_nat c h1 result == toDomain_ #c ((-3) * fromDomain_ #c (as_nat c h0 a) % getPrime c) /\
+    as_nat c h1 result == toDomain_ #c ((-3) * fromDomain_ #c (as_nat c h0 a)))
