code/ecdsap256/Hacl.Impl.P256.PointAdd.fsti
@@ -31,34 +31,32 @@ open FStar.Mul
 
 #reset-options "--z3rlimit 300" 
 
-(*)
-val point_add: p: point -> q: point -> result: point -> tempBuffer: lbuffer uint64 (size 88) -> 
+val point_add: #c: curve -> p: point c -> q: point c -> result: point c -> tempBuffer: lbuffer uint64 (size 88) -> 
    Stack unit (requires fun h -> live h p /\ live h q /\ live h result /\ live h tempBuffer /\ 
    eq_or_disjoint q result /\
    disjoint p q /\ disjoint p tempBuffer /\ disjoint q tempBuffer /\ disjoint p result /\ disjoint result tempBuffer /\  
-    as_nat h (gsub p (size 8) (size 4)) < prime256 /\ 
-    as_nat h (gsub p (size 0) (size 4)) < prime256 /\ 
-    as_nat h (gsub p (size 4) (size 4)) < prime256 /\
-    as_nat h (gsub q (size 8) (size 4)) < prime256 /\ 
-    as_nat h (gsub q (size 0) (size 4)) < prime256 /\  
-    as_nat h (gsub q (size 4) (size 4)) < prime256 
+    as_nat c h (gsub p (size 8) (size 4)) < prime256 /\ 
+    as_nat c h (gsub p (size 0) (size 4)) < prime256 /\ 
+    as_nat c h (gsub p (size 4) (size 4)) < prime256 /\
+    as_nat c h (gsub q (size 8) (size 4)) < prime256 /\ 
+    as_nat c h (gsub q (size 0) (size 4)) < prime256 /\  
+    as_nat c h (gsub q (size 4) (size 4)) < prime256 
     ) 
    (ensures fun h0 _ h1 -> 
      modifies (loc tempBuffer |+| loc result) h0 h1 /\ 
-     as_nat h1 (gsub result (size 8) (size 4)) < prime256 /\ 
-     as_nat h1 (gsub result (size 0) (size 4)) < prime256 /\ 
-     as_nat h1 (gsub result (size 4) (size 4)) < prime256 /\
+     as_nat c h1 (gsub result (size 8) (size 4)) < prime256 /\ 
+     as_nat c h1 (gsub result (size 0) (size 4)) < prime256 /\ 
+     as_nat c h1 (gsub result (size 4) (size 4)) < prime256 /\
      (
        let pX, pY, pZ = gsub p (size 0) (size 4), gsub p (size 4) (size 4), gsub p (size 8) (size 4) in 
        let qX, qY, qZ = gsub q (size 0) (size 4), gsub q (size 4) (size 4), gsub q (size 8) (size 4) in 
        let x3, y3, z3 = gsub result (size 0) (size 4), gsub result (size 4) (size 4), gsub result (size 8) (size 4) in 
        
-       let pxD, pyD, pzD = fromDomain_ (as_nat h0 pX), fromDomain_ (as_nat h0 pY), fromDomain_ (as_nat h0 pZ) in 
-       let qxD, qyD, qzD = fromDomain_ (as_nat h0 qX), fromDomain_ (as_nat h0 qY), fromDomain_ (as_nat h0 qZ) in 
-       let x3D, y3D, z3D = fromDomain_ (as_nat h1 x3), fromDomain_ (as_nat h1 y3), fromDomain_ (as_nat h1 z3) in
+       let pxD, pyD, pzD = fromDomain_ #c (as_nat c h0 pX), fromDomain_ #c (as_nat c h0 pY), fromDomain_ #c (as_nat c h0 pZ) in 
+       let qxD, qyD, qzD = fromDomain_ #c (as_nat c h0 qX), fromDomain_ #c (as_nat c h0 qY), fromDomain_ #c (as_nat c h0 qZ) in 
+       let x3D, y3D, z3D = fromDomain_ #c (as_nat c h1 x3), fromDomain_ #c (as_nat c h1 y3), fromDomain_ #c (as_nat c h1 z3) in
       
-       let xN, yN, zN = _point_add #P256 (pxD, pyD, pzD) (qxD, qyD, qzD) in 
+       let xN, yN, zN = _point_add #c (pxD, pyD, pzD) (qxD, qyD, qzD) in 
        x3D == xN /\ y3D == yN /\ z3D == zN
   )
 )
- *)
